cryptographically fix Model.AEAD.encrypt

src/tls/Model.AEAD.fst
@@ -83,7 +83,8 @@ let is_fresh_iv
 
 let encrypt
   #a #phi s iv plain
-= let cipher = SC.encrypt (state_kv s) iv Seq.empty plain in
+= let plain' = if F.ideal_AEAD then Seq.create (Seq.length plain) (Crypto.Util.IntCast.to_sec8 0uy) else plain in
+  let cipher = SC.encrypt (state_kv s) iv Seq.empty plain' in
   if F.ideal_iv
   then begin
     let h = HST.get () in
@@ -92,10 +93,9 @@ let encrypt
     let h' = HST.get () in
     B.modifies_loc_regions_intro (Set.singleton (HS.frameOf tbl)) h h' ;
     B.modifies_loc_addresses_intro (HS.frameOf tbl) (Set.singleton (HS.as_addr tbl)) B.loc_none h h' ;
-    assume (HST.equal_domains h h'); // TODO: fix FStar.Monotonic.DependentMap
-    if F.ideal_AEAD then Seq.create (SC.cipher_length plain) (Crypto.Util.IntCast.to_sec8 0uy) else cipher
-  end else
-    cipher
+    assume (HST.equal_domains h h') // TODO: fix FStar.Monotonic.DependentMap
+  end;
+  cipher
 
 let decrypt
   #a #phi s iv cipher
